cleaned and refactored some proofs

src/Rdf.v
@@ -5,7 +5,7 @@ Unset Printing Implicit Defensive.
 From RDF Require Import Term.
 From RDF Require Import Triple.
 
-Section rdf.
+Section Rdf.
   Variable I B L: eqType.
   Let term:= (term I B L).
   Let triple:= (triple I B L).
@@ -42,47 +42,49 @@ Section rdf.
     have eqsib: sib2 = (eq_ir geq sib1);
       have eqpi : pi2 = (eq_ir geq pi1);
       have eqoibl: oibl2 = (eq_ir geq oibl1); try apply eq_irrelevance.
-    rewrite eqsib eqpi eqoibl. erewrite <-geq. f_equal; apply eq_irrelevance. 
+    rewrite eqsib eqpi eqoibl. erewrite <-geq. f_equal; by apply eq_irrelevance. 
   Qed.
   
   Definition rdf_eqP : Equality.axiom eqb_rdf.
   Proof. rewrite /Equality.axiom => x y.
-         apply: (iffP idP) => //= [| ->]; case: x y=> [g1 sib1 pi1 oibl1] [g2 sib2 pi2 oibl2]. apply graph_inj. apply eqb_rdf_refl. 
+         apply: (iffP idP) => //= [| ->];
+                             case: x y=> [g1 sib1 pi1 oibl1] [g2 sib2 pi2 oibl2]. apply graph_inj. by apply eqb_rdf_refl.
   Qed.
 
-  Definition relabeling_seq_triple (μ : B -> B) (g : seq triple) : seq triple :=
-    map (relabeling_triple μ) g.
+  Definition relabeling_seq_triple (μ : B -> B) (g : seq triple) : seq triple := map (relabeling_triple μ) g.
 
   Lemma relabeling_seq_triple_id (g : seq triple) : relabeling_seq_triple id g = g.
-  Proof. rewrite /relabeling_seq_triple. apply /eqP. elim g => [//|h t /eqP iht] /=. rewrite relabeling_triple_id. by rewrite iht. Qed.
+  Proof. rewrite /relabeling_seq_triple. apply /eqP.
+         elim g => [//|h t /eqP iht] /=. rewrite relabeling_triple_id. by rewrite iht. Qed.
 
   Lemma relabeling_seq_triple_comp_simpl (g : seq triple) (μ12 μ23 : B -> B) :
     relabeling_seq_triple (μ23 \o μ12) g = (relabeling_seq_triple μ23 \o (relabeling_seq_triple μ12)) g.
-  Proof. rewrite /relabeling_seq_triple /=. elim g => [//|h t iht] /=. rewrite relabeling_triple_comp /=. f_equal; apply iht.
+  Proof. rewrite /relabeling_seq_triple /=.
+         elim g => [//|h t iht] /=. rewrite relabeling_triple_comp /=. by f_equal; apply iht.
   Qed.
 
   Lemma relabeling_seq_triple_comp_P (g1 g2 : seq triple) (eqb : g1 = g2) (μ : B->B) :
     relabeling_seq_triple μ g1 = relabeling_seq_triple μ g2. by rewrite eqb. Qed.
 
   Lemma relabeling_seq_triple_comp (μ1 μ2 : B -> B) (g : seq triple) : relabeling_seq_triple μ1 (relabeling_seq_triple μ2 g) = (relabeling_seq_triple μ1 \o (relabeling_seq_triple μ2)) g.
-    Proof. by []. Qed. 
+  Proof. by []. Qed. 
 
   Lemma relabeling_seq_triple_preserves_subject_in_IB (g : seq triple) (μ : B -> B) :
     all (fun t => is_in_ib (subject t)) g ->
     all (fun t => is_in_ib (subject t)) (relabeling_seq_triple μ g).
-  Proof. move=> /allP sin. apply /allP => [[s p o /= sint pint oint]] => tg. apply sint. 
+  Proof. move=> /allP sin. apply /allP => [[s p o /= sint pint oint]] => tg. by apply sint. 
   Qed.
 
   Lemma relabeling_seq_triple_preserves_predicate_in_I (g : seq triple) (μ : B -> B) :
     all (fun t => is_in_i (predicate t)) g ->
     all (fun t => is_in_i (predicate t)) (relabeling_seq_triple μ g).
-  Proof. move=> /allP pin. apply /allP => [[s p o /= sint pint oint]] => tg . apply pint.
+  Proof. move=> /allP pin. apply /allP => [[s p o /= sint pint oint]] => tg. by apply pint.
   Qed.
 
   Lemma relabeling_seq_triple_preserves_object_in_IBL (g : seq triple) (μ : B -> B) :
     all (fun t => is_in_ibl (object t)) g ->
     all (fun t => is_in_ibl (object t)) (relabeling_seq_triple μ g).
-  Proof. move=> /allP oin. apply /allP => [[s p o /= sibt pibt oint]] => tg . apply oint.
+  Proof. move=> /allP oin. apply /allP => [[s p o /= sibt pibt oint]] => tg. by apply oint.
   Qed.
 
   Definition relabeling (μ : B -> B) (g : rdf_graph): rdf_graph :=
@@ -116,12 +118,6 @@ Section rdf.
          by rewrite relabeling_id eqb_rdf_refl.
   Qed.
 
-  (* Definition inv (bij : Type) : bijective : bijective f := *)
-
-  (*    Inductive ubn_geq_spec m : nat -> Type := *)
-  (*   UbnGeq n of n <= m : ubn_geq_spec m n. *)
-  (* Lemma ubnPgeq m : ubn_geq_spec m m. *)
-  (* Proof. by []. Qed. *)
   Lemma relabelingG_ext (μ1 μ2 : B -> B) : μ1 =1 μ2 -> forall g, relabeling_seq_triple μ1 g = relabeling_seq_triple μ2 g.
   Proof. move => μpqeq. elim=> [//|h t IHt] /=. rewrite IHt. f_equal. by apply relabeling_triple_ext. Qed.
 
@@ -129,31 +125,29 @@ Section rdf.
   Proof. move=> μpweq g. apply /graph_inj. rewrite /eqb_rdf. case g. rewrite /= => gs _ _ _. apply /eqP. by apply relabelingG_ext. Qed.
 
   Lemma relabeling_comp_simpl (μ1 μ2 : B -> B) (g : rdf_graph) : relabeling μ1 (relabeling μ2 g) = relabeling (μ1 \o μ2) g.
-    Proof. by rewrite -relabeling_comp. Qed.
+  Proof. by rewrite -relabeling_comp. Qed.
 
   Lemma bijective_eqb_rdf mu nu g1 g2 : cancel mu nu -> eqb_rdf g1 (relabeling mu g2) ->  eqb_rdf g2 (relabeling nu g1).
   Proof.
-  move=> cancel_mu_nu /graph_inj->.
-  rewrite relabeling_comp_simpl.
-  have /relabeling_ext-> : nu \o mu =1 id by [].
-  rewrite relabeling_id; exact: eqb_rdf_refl.
+    move=> cancel_mu_nu /graph_inj->.
+    rewrite relabeling_comp_simpl.
+    have /relabeling_ext-> : nu \o mu =1 id by [].
+    rewrite relabeling_id; exact: eqb_rdf_refl.
   Qed.  
 
   Lemma iso_symm (g1 g2 : rdf_graph) :
-      iso g1 g2 <-> iso g2 g1.
+    iso g1 g2 <-> iso g2 g1.
   Proof.
     rewrite /iso /is_iso.
     split; case=> mu [mu_bij heqb_rdf]; case: (mu_bij)=> [nu h1 h2];
-          (exists nu; split; [exact: bij_can_bij h1 | exact: bijective_eqb_rdf heqb_rdf]).
+                                                       (exists nu; split; [exact: bij_can_bij h1 | exact: bijective_eqb_rdf heqb_rdf]).
   Qed. 
 
-
- Lemma iso_trans (g1 g2 g3: rdf_graph) : iso g1 g2 -> iso g2 g3 -> iso g1 g3.
+  Lemma iso_trans (g1 g2 g3: rdf_graph) : iso g1 g2 -> iso g2 g3 -> iso g1 g3.
   Proof. rewrite /iso /is_iso=> [[μ1 [bij1 /graph_inj eqb1]] [μ2 [bij2 /graph_inj eqb2]]].
          exists (μ1 \o μ2). split. 
          rewrite /=. apply bij_comp. apply bij1. apply bij2.
          rewrite -relabeling_comp /= -eqb2 -eqb1. by apply eqb_rdf_refl.
- Qed.
+  Qed.
 
-End rdf.
-
+End Rdf.
